metacoq_erasure test

benchmarks/metacoq_erasure.v
@@ -8,27 +8,142 @@ From CertiCoq.Plugin Require Import CertiCoq.
 
 Open Scope string.
 
-From MetaCoq.Erasure Require Import Erasure Loader.
-From MetaCoq.Template Require Import MCString.
+From MetaCoq.Erasure Require Import ERemoveParams Erasure Loader.
+From MetaCoq.Template Require Import MCString EtaExpand.
+From MetaCoq.PCUIC Require Import TemplateToPCUIC.
 
-Program Definition erase (p : Ast.Env.program) : eprogram :=
+From CertiCoq.Benchmarks Require Import ErasureFunction.
+
+Import Transform.
+
+Program Definition erase_pcuic_program (p : pcuic_program) 
+  (wfΣ : ∥ PCUICTyping.wf_ext (H := config.extraction_checker_flags) p.1 ∥)
+  (wt : ∥ ∑ T, PCUICTyping.typing (H := config.extraction_checker_flags) p.1 [] p.2 T ∥) : eprogram_env :=
+  let wfe := build_wf_env_from_env p.1.1 (map_squash (wf_ext_wf _) wfΣ) in
+  let wfe' := make_wf_env_ext wfe p.1.2 wfΣ in
+  let t := ErasureFunction.erase wfe' nil p.2 _ in
+  let Σ' := ErasureFunction.erase_global (EAstUtils.term_global_deps t) wfe in
+  (EEtaExpanded.GlobalContextMap.make Σ' _, t).
+  
+Next Obligation.
+  sq. destruct wt as [T Ht].
+  cbn. now exists T.
+Qed.
+Next Obligation.
+  unfold erase_global.
+  eapply wf_glob_fresh. todo "wf".
+Qed.
+
+Obligation Tactic := idtac.
+
+Program Definition erase_transform : Transform.t pcuic_program eprogram_env PCUICAst.term EAst.term eval_pcuic_program (eval_eprogram_env EWcbvEval.default_wcbv_flags) :=
+ {| name := "erasure";
+    pre p :=  
+      ∥ PCUICTyping.wf_ext (H := config.extraction_checker_flags) p.1 ×
+       ∑ T, PCUICTyping.typing (H := config.extraction_checker_flags) p.1 [] p.2 T ∥;
+    transform p hp := erase_pcuic_program p (map_squash fst hp) (map_squash snd hp) ;
+    post p := true;
+    obseq g g' v v' := True |}.
+Next Obligation.
+  intros [Σ t] [[wfext ht]]. exact eq_refl.
+Qed.
+Next Obligation.
+  red. intros. todo "eval".
+Qed.
+
+Import Transform.
+Local Notation " o ▷ o' " := (Transform.compose o o' _) (at level 50, left associativity).
+
+Local Existing Instance config.default_checker_flags.
+
+Program Definition erasure_pipeline := 
+  template_to_pcuic_transform ▷
+  pcuic_expand_lets_transform ▷
+  erase_transform.
+  (* ▷ 
+  remove_params_fast_optimization _ ▷  *)
+Next Obligation.
+  intros. todo "foo".
+Qed.
+Next Obligation.
+  intros. todo "foo".
+Qed.
+Definition erase_program_aux := Transform.run erasure_pipeline.
+
+Definition eta_global_env (g : global_env) := 
+  {| universes := g.(universes); declarations := eta_global_env g.(declarations) |}.
+
+Definition eta_program p := 
+  let Σ' := eta_global_env p.1 in 
+  (Σ', eta_expand Σ'.(declarations) p.2).
+
+Definition erase_program p := erase_program_aux (eta_program p).
+
+Program Definition erase (p : Ast.Env.program) : eprogram_env :=
   erase_program p (MCUtils.todo "wf_env and welltyped term").
 
 Program Definition erase_and_print_template_program (p : Ast.Env.program) : string :=
   let (Σ', t) := erase_program p (MCUtils.todo "wf_env and welltyped term") in
+  let Σ' := EEtaExpanded.GlobalContextMap.global_decls Σ' in
   (EPretty.print_term Σ' nil true false t ++ nl ++ "in:" ++ nl ++ EPretty.print_global_context Σ')%string.
 
-MetaCoq Erase true.
+(* Program Definition erase_and_print_template_program (p : Ast.Env.program) : string := *)
+  (* let (Σ', t) := erase_program p (MCUtils.todo "wf_env and welltyped term") in *)
+  (* (PCUICPretty.print_term (TemplateToPCUIC.global_env_ext_map_global_env_ext Σ') false [] true false t ++ nl ++ "in:" ++ nl). *)
+   (* PCUICPretty.print_global_env Σ')%string. *)
 
-MetaCoq Quote Recursively Definition foo := (true, false).
-(* ((fun (X : Set) (x : X) (e : x = x) => *)
-                  (* match e in eq _ x' return bool with *)
-                  (* | eq_refl => true *)
-                  (* end)). *)
+(* MetaCoq Erase is_arity. *)
 
-Definition metacoq_erasure := (erase_and_print_template_program foo).
+From Equations Require Import Equations.
 
-CertiCoq Compile -O 0 -debug metacoq_erasure.
+Equations wf_fix (n : nat) (H : n > 0): nat
+  by wf n lt :=
+  | 0, _ := 1
+  | S n, _ := S (wf_fix n _).
+Next Obligation. todo "bla". Qed.
+
+MetaCoq Quote Recursively Definition foo := (List.map (fun x => negb x) [true]).
+MetaCoq Quote Recursively Definition footy := (ltac:(let ty := type of prod in exact ty)).
+
+Program Definition to_pcuic_pipeline := 
+  template_to_pcuic_transform ▷
+  pcuic_expand_lets_transform.
+(* Next Obligation.
+  intros. todo "foo".
+Qed. *)
+
+Definition to_pcuic_aux := Transform.run to_pcuic_pipeline.
+
+Axiom (print_nat : nat -> unit).
+
+Axiom sorry : forall {A : Prop}, A.
+Local Existing Instance PCUICSN.extraction_normalizing.
+Import PCUICErrors PCUICWfEnv.
+Definition reduce_to_sort_test := 
+  let p := to_pcuic_aux footy (MCUtils.todo "precondition") in
+  let wfe := build_wf_env_from_env p.1.1 sorry in
+  let wfe' := make_wf_env_ext wfe p.1.2 sorry in
+  match PCUICSafeReduce.reduce_to_sort wfe' [] p.2 sorry with
+  | Checked_comp s => string_of_sort s.π1
+  | TypeError_comp _ _ => 
+    let _ := ErasureFunction.pr_term "not a sort" wfe' [] p.2 in "not a sort"
+  end.
+
+(* Definition metacoq_erasure := reduce_to_sort_test. *)
+Definition metacoq_erasure := (erase_and_print_template_program foo). 
+(* Definition metacoq_erasure := 
+  let _ := print_str "metacoq_erasure" in
+  let _ := print_newline tt in
+  print_nat (wf_fix (S (S 0)) sorry). *)
+
+(* MetaCoq Erase wf_fix.   *)
+(* Eval lazy in metacoq_erasure. *)
+CertiCoq Compile -O 0 metacoq_erasure
+Extract Constants [ 
+  (* print_nat => "print_gallina_nat", *)
+  CertiCoq.Benchmarks.ErasureFunction.print_str => "print_gallina_string",
+  CertiCoq.Benchmarks.ErasureFunction.print_newline => "print_new_line" ] 
+Include [ "print.h" ]. 
 (*
 Definition er := Eval lazy in erase foo.
 
